Proved some results on Thompson Construction

Regex/NFA/Compile.lean
@@ -1,47 +1,175 @@
 import Regex.Regex
 import Regex.NFA.Basic
 
+import Mathlib.Tactic.Common
+
 namespace NFA
 
-def addNode (nodes : Array Node) (node : Node) : Array Node × Nat :=
-  let nodes := nodes.push node
-  (nodes, nodes.size - 1)
+def addNode (nodes : Array Node) (node : Node) :
+  (nodes' : { nodes' : Array Node // nodes.size < nodes'.size}) ×
+  { i : Fin nodes'.val.size // i = nodes.size } :=
+  have lt_size : nodes.size < (nodes.push node).size := by
+    simp [Array.size_push]
+  have isLt : nodes.size < (nodes.push node).size := by
+    simp [Array.size_push]
+  ⟨⟨nodes.push node, lt_size⟩, ⟨⟨nodes.size, isLt⟩, rfl⟩⟩
+
+theorem addNode.get_lt {nodes : Array Node} {node : Node} {i : Nat} (h : i < nodes.size) :
+  (addNode nodes node).1.val[i]'(Nat.lt_trans h (addNode nodes node).1.property) = nodes[i] := by
+  simp [addNode]
+  apply Array.get_push_lt
+
+@[simp]
+theorem addNode.get_node {nodes : Array Node} {node : Node} :
+  (addNode nodes node).1.val[(addNode nodes node).2.val] = node := by
+  show (addNode nodes node).1.val[(addNode nodes node).2.val.val] = node
+  simp [addNode]
 
 /--
   Thompson construction algorithm for converting the given regex to NFA.
 -/
-def compileRaw (r : Regex) : Array Node × Nat :=
-  loop #[.done] 0 r
+def compileRaw (r : Regex) :
+  (nodes : Array Node) × Fin nodes.size :=
+  let result := loop #[.done] 0 r
+  ⟨result.1.val, result.2⟩
 where
   /--
     The main loop of the compilation.
 
-    It compiles the regex `r` into the given `nodes`. The compiled nodes transition to `next`
-    if the input matches. It returns the new `nodes` and the corresponding ID for `r` in the array.
+    It compiles the given regex into the given `nodes`. The compiled nodes transition to `next`
+    if and only if the input matches. It returns the new `nodes` and the corresponding ID for the
+    given regex in the array.
   -/
-  loop (nodes : Array Node) (next : Nat) : Regex → Array Node × Nat
-  | .empty => addNode nodes .fail
-  | .epsilon => addNode nodes (.epsilon next)
-  | .char c => addNode nodes (.char c next)
+  loop (nodes : Array Node) (next : Nat) :
+    Regex → (nodes' : { nodes' : Array Node // nodes.size < nodes'.size}) × Fin nodes'.val.size
+  | .empty =>
+    let ⟨nodes, start⟩ := addNode nodes .fail
+    ⟨nodes, start.val⟩
+  | .epsilon =>
+    let ⟨nodes, start⟩ := addNode nodes (.epsilon next)
+    ⟨nodes, start.val⟩
+  | .char c =>
+    let ⟨nodes, start⟩ := addNode nodes (.char c next)
+    ⟨nodes, start.val⟩
   | .alternate r₁ r₂ =>
-    let (nodes, target₁) := loop nodes next r₁
-    let (nodes, target₂) := loop nodes next r₂
-    addNode nodes (.split target₁ target₂)
+    let ⟨nodes₁, start₁⟩ := loop nodes next r₁
+    let ⟨nodes₂, start₂⟩ := loop nodes₁ next r₂
+    let ⟨nodes', start⟩ := addNode nodes₂ (.split start₁ start₂)
+
+    have property : nodes.size < nodes'.val.size :=
+      calc nodes.size
+        _ < nodes₁.val.size := nodes₁.property
+        _ < nodes₂.val.size := nodes₂.property
+        _ < nodes'.val.size := nodes'.property
+
+    ⟨⟨nodes', property⟩, start⟩
   | .concat r₁ r₂ =>
-    let (nodes, next) := loop nodes next r₂
-    loop nodes next r₁
+    let ⟨nodes₂, start₂⟩ := loop nodes next r₂
+    let ⟨nodes₁, start₁⟩ := loop nodes₂ start₂ r₁
+
+    have property : nodes.size < nodes₁.val.size :=
+      calc nodes.size
+        _ < nodes₂.val.size := nodes₂.property
+        _ < nodes₁.val.size := nodes₁.property
+
+    ⟨⟨nodes₁, property⟩, start₁⟩
   | .star r =>
     -- We need to generate a placeholder node first. We use `done` for it to save an allocation.
     -- TODO: check generated code
-    let (nodes, start) := addNode nodes .done
-    let (nodes, target) := loop nodes start r
-    -- Patch the placeholder node
-    -- TODO: prove in-bounds? It might be sufficient to use setD.
-    let nodes := nodes.set! start (.split target next)
-    (nodes, start)
+    let ⟨nodes', ⟨start, _⟩⟩ := addNode nodes .done
+    let ⟨nodes'', target⟩ := loop nodes' start r
 
-#eval compileRaw (Regex.star (Regex.char 'a'))
-#eval compileRaw (Regex.alternate (Regex.char 'a') (Regex.star (Regex.concat (Regex.char 'a') (Regex.char 'b'))))
-#eval compileRaw (Regex.alternate Regex.empty (Regex.concat (Regex.char 'a') Regex.empty))
+    have property : nodes.size < nodes''.val.size :=
+      calc nodes.size
+        _ < nodes'.val.size := nodes'.property
+        _ < nodes''.val.size := nodes''.property
+    have isLt : start.val < nodes''.val.size :=
+      calc start.val
+        _ < nodes'.val.size := start.isLt
+        _ < nodes''.val.size := nodes''.property
+
+    -- Patch the placeholder node
+    let nodes''' := nodes''.val.set ⟨start.val, isLt⟩ (.split target next)
+
+    have eq_size : nodes'''.size = nodes''.val.size := by simp
+    have isLt : start.val < nodes'''.size := by
+      rw [eq_size]
+      exact isLt
+
+    ⟨⟨nodes''', eq_size ▸ property⟩, ⟨start.val, isLt⟩⟩
+
+def compileRaw.loop.get_lt {i : Nat} (h : i < nodes.size) :
+  (loop nodes next r).1.val[i]'(Nat.lt_trans h (loop nodes next r).1.property) = nodes[i] := by
+  -- have isLt := Nat.lt_trans h (loop nodes next r).1.property
+  induction r generalizing nodes next with
+  | empty | epsilon | char c => simp [loop]; apply addNode.get_lt
+  | alternate r₁ r₂ ih₁ ih₂ =>
+    let result₁ := loop nodes next r₁
+    let result₂ := loop result₁.1 next r₂
+    let result := addNode result₂.1 (.split result₁.2 result₂.2)
+
+    have isLt₁ : i < result₁.1.val.size := Nat.lt_trans h result₁.1.property
+    have isLt₂ : i < result₂.1.val.size := Nat.lt_trans isLt₁ result₂.1.property
+    have isLt : i < result.1.val.size := Nat.lt_trans isLt₂ result.1.property
+
+    show result.1.val[i] = nodes[i]
+
+    calc result.1.val[i]
+      _ = result₂.1.val[i] := addNode.get_lt isLt₂
+      _ = result₁.1.val[i] := ih₂ isLt₁
+      _ = nodes[i] := ih₁ h
+  | concat r₁ r₂ ih₁ ih₂ =>
+    let result₂ := loop nodes next r₂
+    let result₁ := loop result₂.1 result₂.2 r₁
+
+    have isLt₂ : i < result₂.1.val.size := Nat.lt_trans h result₂.1.property
+    have isLt₁ : i < result₁.1.val.size := Nat.lt_trans isLt₂ result₁.1.property
+
+    show result₁.1.val[i] = nodes[i]
+
+    calc result₁.1.val[i]
+      _ = result₂.1.val[i] := ih₁ isLt₂
+      _ = nodes[i] := ih₂ h
+  | star r ih =>
+    let result := addNode nodes .done
+    let result' := loop result.1 result.2 r
+
+    have property : nodes.size < result'.1.val.size :=
+      calc nodes.size
+        _ < result.1.val.size := result.1.property
+        _ < result'.1.val.size := result'.1.property
+    have startIsLt : result.2.val.val < result'.1.val.size :=
+      calc result.2.val.val
+        _ < result.1.val.size := result.2.val.isLt
+        _ < result'.1.val.size := result'.1.property
+
+    let nodes' := result'.1.val.set ⟨result.2.val, startIsLt⟩ (.split result'.2 next)
+
+    have eq_size : nodes'.size = result'.1.val.size := by simp
+
+    have isLt : i < result.1.val.size := Nat.lt_trans h result.1.property
+    have isLt' : i < result'.1.val.size := Nat.lt_trans isLt result'.1.property
+    have isLt'' : i < nodes'.size := eq_size ▸ Nat.lt_trans h startIsLt
+
+    show nodes'[i] = nodes[i]
+
+    calc nodes'[i]
+      _ = result'.1.val[i] := by
+        rw [Array.get_set_ne]
+        exact Nat.ne_of_gt (result.2.property.symm ▸ h)
+      _ = result.1.val[i] := ih isLt
+      _ = nodes[i] := addNode.get_lt h
+
+def compile (r : Regex) : NFA :=
+  let result := compileRaw r
+  let nodes := result.1
+  let start := result.2
+
+  -- TODO: inBoundsはNatを受け取った方が証明が楽そう。nodesの内容を見ないで良いため
+  ⟨nodes, start, sorry⟩
+
+#eval compile (Regex.star (Regex.char 'a'))
+#eval compile (Regex.alternate (Regex.char 'a') (Regex.star (Regex.concat (Regex.char 'a') (Regex.char 'b'))))
+#eval compile (Regex.alternate Regex.empty (Regex.concat (Regex.char 'a') Regex.empty))
 
 end NFA
